ironfleet/src/IronRaftClient/RaftClient.cs
@@ -1,0 +1,102 @@
+using IronfleetIoFramework;
+using System;
+using System.Collections.Generic;
+using System.IO;
+using System.Linq;
+using System.Net;
+
+namespace IronRaftClient
+{
+  public class RaftClient
+  {
+    ServiceIdentity serviceIdentity;
+    byte[][] serverPublicKeys;
+    bool verbose;
+    UInt64 nextSeqNum;
+    int primaryServerIndex;
+    IoScheduler scheduler;
+
+    public RaftClient(ServiceIdentity i_serviceIdentity, string serviceName, bool i_verbose)
+    {
+      serviceIdentity = i_serviceIdentity;
+      if (serviceIdentity.ServiceType != "IronRaft" + serviceName) {
+        Console.Error.WriteLine("Provided service identity has type {0}, not IronRaft{1}.",
+                                serviceIdentity.ServiceType, serviceName);
+        throw new Exception("Wrong service type");
+      }
+      serverPublicKeys = serviceIdentity.Servers.Select(server => IoScheduler.HashPublicKey(server.PublicKey)).ToArray();
+      verbose = i_verbose;
+      nextSeqNum = 0;
+      primaryServerIndex = 0;
+      scheduler = IoScheduler.CreateClient(serviceIdentity.Servers, verbose, /*serviceIdentity.UseSsl*/false);
+    }
+
+    public byte[] SubmitRequest (byte[] request, int timeBeforeServerSwitchMs = 1000)
+    {
+      UInt64 seqNum = nextSeqNum++;
+      byte[] requestMessage;
+      using (var memStream = new MemoryStream())
+      {
+        IoEncoder.WriteUInt64(memStream, 4);                                 // 4 means "this is a CMessage_Request"
+        IoEncoder.WriteUInt64(memStream, seqNum);                            // sequence number
+        IoEncoder.WriteUInt64(memStream, (UInt64)request.Length);            // size of CAppRequest
+        IoEncoder.WriteBytes(memStream, request, 0, (UInt64)request.Length); // CAppRequest
+        requestMessage = memStream.ToArray();
+      }
+
+      scheduler.SendPacket(serverPublicKeys[primaryServerIndex], requestMessage);
+      if (verbose) {
+        Console.WriteLine("Sending a request with sequence number {0} to {1}",
+                          seqNum, serviceIdentity.Servers[primaryServerIndex]);
+      }
+
+      while (true)
+      {
+        bool ok, timedOut;
+        byte[] remote;
+        byte[] replyBytes;
+        scheduler.ReceivePacket(timeBeforeServerSwitchMs, out ok, out timedOut, out remote, out replyBytes);
+
+        if (!ok) {
+          throw new Exception("Unrecoverable networking failure");
+        }
+
+        if (timedOut) {
+          // primaryServerIndex = (primaryServerIndex + 1) % serviceIdentity.Servers.Count();
+          if (verbose) {
+            Console.WriteLine("#timeout; rotating to server {0}", primaryServerIndex);
+          }
+          scheduler.SendPacket(serverPublicKeys[primaryServerIndex], requestMessage);
+          continue;
+        }
+
+        if (replyBytes.Length < 24) {
+          throw new Exception(String.Format("Got Raft reply with invalid length {0}", replyBytes.Length));
+        }
+
+        UInt64 messageType = IoEncoder.ExtractUInt64(replyBytes, 0);
+        if (messageType != 5) {
+          throw new Exception("Got Raft message that wasn't a reply");
+        }
+
+        UInt64 replySeqNum = IoEncoder.ExtractUInt64(replyBytes, 8);
+        if (replySeqNum != seqNum) {
+          // This is a retransmission of a reply for an old sequence
+          // number.  Ignore it.
+          continue;
+        }
+
+        UInt64 replyOk = IoEncoder.ExtractUInt64(replyBytes, 16);
+        UInt64 leader_id = IoEncoder.ExtractUInt64(replyBytes, 24);
+        UInt64 replyLength = IoEncoder.ExtractUInt64(replyBytes, 32);
+        if (replyLength + 40 != (UInt64)replyBytes.Length) {
+          throw new Exception(String.Format("Got Raft reply with invalid encoded length ({0} instead of {1})",
+                                            replyLength, replyBytes.Length - 24));
+        }
+
+        Console.WriteLine("\033[1;32mGot reply from server {0}\033[0m", leader_id);
+        return replyBytes.Skip(24).ToArray();
+      }
+    }
+  }
+}
