ironfleet/src/Dafny/Distributed/Protocol/Raft/Types.i.dfy
@@ -24,6 +24,8 @@ datatype RaftMessage =
   | RaftMessage_RequestVoteReply(term:int, vote_granted:bool)
   | RaftMessage_AppendEntries(term:int, leader_ep:EndPoint, prev_log_index:int, prev_log_term:int, entries:seq<LogEntry>, leader_commit:int)
   | RaftMessage_AppendEntriesReply(term:int, success:bool, match_index:int)
+  | RaftMessage_Request(seqno_req:int, req:AppRequest)
+  | RaftMessage_Reply(seqno_reply:int, reply:AppReply, ok:bool, leader_id:int)
 
 datatype RaftRole = Follower | Candidate | Leader
 
