ironfleet/weekly_summary.md
@@ -1,0 +1,25 @@
+#### Last Week
+
+- Impl:
+  - message parsing and marshaling
+    - grammar
+    - demarshal (bytearray -> datatype)
+    - define marshallable (all kinds of sizes should be limited) and valid (semantically valid)
+    - marshal (datatype -> bytearray)
+  - NetRaft.i.dfy: 
+    - marshal and send Raft Package
+    - receive and demarshall to Raft Package
+  - actions:
+    - action0: general receiving, reading clock, and replying
+      - if follower receives heartbeat, reset election timeout 
+    - action1: general timeout checking
+      - if leader: send heartbeat 
+  - Program.cs: the driver for Raft Server
+
+#### Next Week Plan
+
+- implement a simple KV storage service interface
+- implement client request and reply
+- add Client.cs
+- implement `appendEntries` and `appendEntriesReply`
+
